progress on add

Cslib/Computability/Machines/MultiTapeTuring/AddRoutine.lean
@@ -20,66 +20,44 @@ public import Cslib.Computability.Machines.MultiTapeTuring.SequentialCombinator
 public import Cslib.Computability.Machines.MultiTapeTuring.WithTapes
 public import Cslib.Computability.Machines.MultiTapeTuring.IteCombinator
 public import Cslib.Computability.Machines.MultiTapeTuring.EqualRoutine
-public import Cslib.Computability.Machines.MultiTapeTuring.TMWithAuxTapes
 
 namespace Turing
 
 variable [Inhabited α] [Fintype α]
-variable {aux k : ℕ}
+variable {k : ℕ}
 
 namespace Routines
 
-def isZero (i : Fin k.succ) := ite i (pop i <;> push i []) (pop i <;> push i [OneTwo.one])
+def isZero (i : Fin k) := ite i (pop i <;> push i []) (pop i <;> push i [OneTwo.one])
 
 @[simp, grind =]
-theorem isZero_eval_list {k : ℕ} {i : Fin k.succ} {tapes : Fin k.succ → List (List OneTwo)}
-  {h_tapes_i : tapes i ≠ []} :
+theorem isZero_eval_list {k : ℕ} {i : Fin k} {tapes : Fin k → List (List OneTwo)} :
   (isZero i).eval_list tapes = .some (Function.update tapes i (
-    (if (tapes i).head h_tapes_i = [] then [OneTwo.one] else []) :: (tapes i).tail)) := by
-  simp [isZero, ite_eval, h_tapes_i]
+    (if (tapes i).headD [] = [] then [OneTwo.one] else []) :: (tapes i).tail)) := by
+  simp [isZero]
   grind
 
-public def neq {k : ℕ} (q s t : Fin k.succ)
-  (h_neq : q ≠ s := by decide) (h_neq' : q ≠ t := by decide) (h_neq'' : s ≠ t := by decide) :
-  MultiTapeTM k.succ (WithSep OneTwo) :=
-  (eq q s t h_neq h_neq' h_neq'') <;> (isZero ⟨t, by omega⟩)
+public def neq {k : ℕ} (q s t : Fin k)
+  (h_inj : [q, s, t].get.Injective := by decide) :
+  MultiTapeTM k (WithSep OneTwo) := eq q s t <;> isZero t
 
 @[simp, grind =]
-public theorem neq_eval_list {k : ℕ} {q s t : Fin k.succ}
-  {h_neq : q ≠ s} {h_neq' : q ≠ t} {h_neq'' : s ≠ t}
-  {tapes : Fin k.succ → List (List OneTwo)}
-  {h_q_nonempty : tapes q ≠ []} {h_s_nonempty : tapes s ≠ []} :
-  (neq q s t (h_neq := h_neq) (h_neq' := h_neq') (h_neq'' := h_neq'')).eval_list tapes =
+public theorem neq_eval_list {k : ℕ} {q s t : Fin k}
+  {h_inj : [q, s, t].get.Injective}
+  {tapes : Fin k → List (List OneTwo)} :
+  (neq q s t h_inj).eval_list tapes =
     Part.some (Function.update tapes t
-      ((if (tapes q).head h_q_nonempty = (tapes s).head h_s_nonempty then
+      ((if (tapes q).headD [] = (tapes s).headD [] then
         []
       else
         [.one]) :: (tapes t))) := by
-  simp [neq, h_q_nonempty, h_s_nonempty]
+  -- TOOD why do we need to instantiate eq_eval_list here?
+  simp_all [neq, eq_eval_list (h_inj := h_inj)]
 
 /-- Execute `tm` a number of times as given by the first word on tape `i`.
+If tape `i` is empty, do not execute the TM.
 Note that the iteration counter is not directly available to the TM. -/
--- TODO maybe it's easier to require that `aux` is at least 3
-def loop (i : Fin k) (tm : MultiTapeTMWithAuxTapes k aux (WithSep OneTwo)) :
-    MultiTapeTMWithAuxTapes k (max aux 3) (WithSep OneTwo) :=
-  sorry
-  -- let tm := tm.add_aux_tapes 3
-  -- let target : Fin (k + (aux + 3)) := ⟨k, by omega⟩
-  -- let counter : Fin (k + (aux + 3)) := ⟨k.succ, by omega⟩
-  -- let cond : Fin (k + (aux + 3)) := ⟨k.succ.succ, by omega⟩
-  -- (copy (k := k + (aux + 3)) i target (h_neq := by grind) <;>
-  -- push counter [] <;>
-  -- neq target counter cond (by grind) (by grind) (by grind) <;>
-  -- doWhile cond (
-  --   pop cond <;>
-  --   tm.toMultiTapeTM <;>
-  --   succ counter <;>
-  --   neq target counter cond (by grind) (by grind) (by grind)) <;>
-  -- pop cond <;>
-  -- pop counter <;>
-  -- pop target).set_aux_tapes (aux + 3)
-
-def loop' (i : ℕ) {h_i : i < k}
+def loop (i : ℕ) {h_i : i < k}
   (tm : MultiTapeTM k (WithSep OneTwo)) : MultiTapeTM (k + 3) (WithSep OneTwo) :=
   sorry
   -- let target : Fin (k + (aux + 3)) := ⟨aux, by omega⟩
@@ -99,145 +77,61 @@ def loop' (i : ℕ) {h_i : i < k}
 
 
 @[simp]
-theorem loop_eval_list {i : Fin k}
-  {tm : MultiTapeTMWithAuxTapes k aux (WithSep OneTwo)}
-  {tapes : Fin k → List (List OneTwo)}
-  (h_tapes_i : tapes ⟨i, by omega⟩ ≠ []) :
-  (loop i tm).eval_list_aux tapes =
-      ((Part.bind · tm.eval_list_aux)^[dya_inv ((tapes ⟨i, by omega⟩).head h_tapes_i)]
-        (Part.some tapes)) := by
-  sorry
-
-@[simp]
-theorem loop'_eval_list {i : ℕ} {h_i : i < k}
+theorem loop_eval_list {i : ℕ} {h_i : i < k}
   {tm : MultiTapeTM k (WithSep OneTwo)}
-  {tapes : Fin (k + 3) → List (List OneTwo)}
-  (h_tapes_i : tapes ⟨i, by omega⟩ ≠ []) :
-  (loop' i tm (h_i := h_i)).eval_list tapes =
-      (((Part.bind · tm.eval_list)^[dya_inv ((tapes ⟨i, by omega⟩).head h_tapes_i)]
+  {tapes : Fin (k + 3) → List (List OneTwo)} :
+  (loop i tm (h_i := h_i)).eval_list tapes =
+      (((Part.bind · tm.eval_list)^[dya_inv ((tapes ⟨i, by omega⟩).headD [])]
         (Part.some (tapes_take tapes k (by omega))))).map
           fun tapes' => tapes_extend_by tapes' tapes := by
   sorry
 
--- @[simp]
--- theorem loop_eval_list' {i : Fin k}
---   {tm : MultiTapeTM k (WithSep OneTwo)}
---   {tapes : Fin (k + 3) → List (List OneTwo)}
---   (h_tapes_i : tapes ⟨i, by omega⟩ ≠ []) :
---   (loop i tm).eval_list tapes =
---       (Part.bind · (tm.extend (k₂ := k + 3) (by omega)).eval_list)
---       ^[dya_inv ((tapes ⟨i, by omega⟩).head h_tapes_i)]
---       (Part.some tapes) := by
---   sorry
-
-/-- Execute `tm` in a loop as long as running `cond` pushes a non-empty value to the last tape. -/
-def whileCond (cond : MultiTapeTM k.succ (WithSep α)) (tm : MultiTapeTM k (WithSep α)) :
-    MultiTapeTM k.succ (WithSep α) :=
-  let k := ⟨k, by omega⟩
-  cond <;>
-  doWhile k ((pop k) <;> (tm.extend (by omega) <;> cond)) <;>
-  (pop ⟨k, by omega⟩)
-
--- lemma whileCond_eval_list {cond : MultiTapeTM k.succ (WithSep α)}
---   {tm : MultiTapeTM k (WithSep α)}
---   {tm_f : Fin k.succ → List (List α) → Option (Fin k.succ → List (List α))}
---   {cond_f : (Fin k.succ → List (List α)) → List α}
---   {h_cond_f : ∀ t, cond.eval_list t = Part.some (Function.update t ⟨k, _⟩ ((cond_f t) :: (t ⟨k, _⟩)))}
---   {tapes : Fin k.succ → List (List α)}
---   {h_nonempty : tapes ⟨k, by omega⟩ ≠ []} :
---   (whileCond cond tm).eval_list tapes =
---     cond.eval_list tapes >>= fun tapes' =>
---       doWhile_eval_list ⟨k, by omega⟩
---         (Function.update tapes' ⟨k, by omega⟩ (tapes' ⟨k, by omega⟩.tail))
---         (pop ⟨k, by omega⟩)
---         (tm.extend (by omega) <;> cond) >>= fun tapes'' =>
---           pop.eval_list tapes'' := by
---   simp [whileCond, seq_eval_list, doWhile_eval_list, pop_eval_list]
---   grind
-
-
--- public def add₀ : MultiTapeTM 4 (WithSep OneTwo) :=
---   copy 1 2 <;> push 1 []
---   -- Here we have [a, 0 :: b, b]
-
--- lemma add₀_eval_list {a b : List OneTwo} {ls₁ ls₂ ls₃ ls₄ : List (List OneTwo)} :
---   add₀.eval_list
---     [a :: ls₁, b :: ls₂, ls₃, ls₄].get =
---     .some [a :: ls₁, [] :: b :: ls₂, b :: ls₃, ls₄].get := by
---   simp [add₀]
---   grind [add₀]
-
 @[simp]
-lemma succ_iter {k r : ℕ} {i : Fin k.succ} {tapes : Fin k.succ → List (List OneTwo)}
-  {h_tapes_i : tapes i ≠ []} :
+lemma succ_iter {k r : ℕ} {i : Fin k.succ} {tapes : Fin k.succ → List (List OneTwo)} :
   (Part.bind · (succ i).eval_list)^[r] (.some tapes) = Part.some (Function.update tapes i (
-    (dya ((dya_inv ((tapes i).head h_tapes_i)) + r)) :: (tapes i).tail)) := by
+    if h : tapes i ≠ [] then
+      (dya ((dya_inv ((tapes i).head h)) + r)) :: (tapes i).tail
+    else
+      tapes i)) := by
   induction r with
-  | zero => simp
-  | succ r ih =>
-    rw [Function.iterate_succ_apply']
-    simp [ih, succ_eval_list]
-    grind
-
-@[simp]
-lemma succ'_iter {k aux r : ℕ} {i : ℕ} {tapes : Fin k → List (List OneTwo)}
-  {h_i_lt : i < k}
-  {h_tapes_i : tapes ⟨i, h_i_lt⟩ ≠ []} :
-  (Part.bind · (succ' (aux := aux) i h_i_lt).eval_list_aux)^[r] (.some tapes) =
-    Part.some (Function.update tapes ⟨i, h_i_lt⟩ (
-      (dya ((dya_inv ((tapes ⟨i, h_i_lt⟩).head h_tapes_i)) + r)) :: (tapes ⟨i, h_i_lt⟩).tail)) := by
-  induction r with
-  | zero => simp
-  | succ r ih =>
-    rw [Function.iterate_succ_apply']
-    simp [ih]
-    grind
+    | zero => simp
+    | succ r ih =>
+      rw [Function.iterate_succ_apply']
+      simp [ih, succ_eval_list]
+      by_cases h_empty : tapes i = []
+      · simp [h_empty]
+      · simp [h_empty]
+        grind
 
 -- Add 0 and 1 and store the result in 2.
+-- Assumes zero for an empty tape.
 public def add₀ : MultiTapeTM 6 (WithSep OneTwo) :=
-  (copy 1 2) <;> loop' (h_i := by decide) 0 (succ (k := 2) 2)
-
-@[simp]
-lemma Function.update_update {α β : Type} [DecidableEq α] {f : α → β} {i : α} {x y : β} :
-  Function.update (Function.update f i x) i y = Function.update f i y := by
-  grind
+  (copy 1 2) <;> loop (h_i := by decide) 0 (succ 2)
 
 @[simp, grind =]
-public theorem add₀_eval_list {tapes : Fin 6 → List (List OneTwo)}
-  {h_nonempty₀ : tapes 0 ≠ []} {h_nonempty₁ : tapes 1 ≠ []} :
+public theorem add₀_eval_list {tapes : Fin 6 → List (List OneTwo)} :
   add₀.eval_list tapes = .some
-    (Function.update tapes 2 ((dya (dya_inv ((tapes 0).head h_nonempty₀) +
-      dya_inv ((tapes 1).head h_nonempty₁)) :: (tapes 2)))) := by
-  simp [add₀, h_nonempty₁, h_nonempty₀]
+    (Function.update tapes 2 ((dya (dya_inv ((tapes 0).headD []) +
+      dya_inv ((tapes 1).headD [])) :: (tapes 2)))) := by
+  simp [add₀]
   grind
 
--- TODO do the 'aux, aux + 1, aux + 2' automatically.
+-- TODO we could also use `k + 3` for aux and thus assume it's always the last `aux` tapes.
 
-public def add {k : ℕ} (i j l aux : ℕ)
-  (h_bounds : i ≠ j ∧ i ≠ l ∧ j ≠ l ∧ i < aux ∧ j < aux ∧ l < aux ∧ aux + 3 ≤ k + 6) :
+public def add (i j l aux : Fin (k + 6))
+  (h_inj : [i, j, l, aux, aux + 1, aux + 2].get.Injective := by decide) :
   MultiTapeTM (k + 6) (WithSep OneTwo) :=
-  add₀.with_tapes #v[
-    ⟨i, by omega⟩, ⟨j, by omega⟩, ⟨l, by omega⟩,
-    ⟨aux, by omega⟩, ⟨aux + 1, by omega⟩, ⟨aux + 2, by omega⟩] (h_le := by omega)
+  add₀.with_tapes [i, j, l, aux, aux + 1, aux + 2].get h_inj
 
 @[simp, grind =]
-public theorem add_eval_list {i j l aux : ℕ}
-  {h_bounds : i ≠ j ∧ i ≠ l ∧ j ≠ l ∧ i < aux ∧ j < aux ∧ l < aux ∧ aux + 3 ≤ k + 6}
-  {tapes : Fin (k + 6) → List (List OneTwo)}
-  {h_nonempty_i : tapes ⟨i, by omega⟩ ≠ []}
-  {h_nonempty_j : tapes ⟨j, by omega⟩ ≠ []} :
-  (add i j l aux h_bounds).eval_list tapes =
-      .some (Function.update tapes ⟨l, by omega⟩ (
-        (dya (dya_inv ((tapes ⟨i, by omega⟩).head h_nonempty_i) +
-          dya_inv ((tapes ⟨j, by omega⟩).head h_nonempty_j)) :: (tapes ⟨l, by omega⟩)))) := by
-  sorry
-
--- TODO remove this? (inline)
-
--- TODO continue here:
--- I think we don't even need eval_list on Aux machines.
--- Check if it works to remove the whole aux machine stuff and instead provide an
--- aux variable explicitly
+public theorem add_eval_list (i j l aux : Fin (k + 6))
+  {h_inj : [i, j, l, aux, aux + 1, aux + 2].get.Injective}
+  {tapes : Fin (k + 6) → List (List OneTwo)} :
+  (add i j l aux h_inj).eval_list tapes =
+      .some (Function.update tapes l (
+        (dya (dya_inv ((tapes i).headD []) + dya_inv ((tapes j).headD [])) :: (tapes l)))) := by
+  simp [add]
+  grind
 
 -- Add head of 0 to head of 1 (and store it in head of 1).
 def add_assign₀' : MultiTapeTM 6 (WithSep OneTwo) :=
