Cslib/Computability/Machines/MultiTapeTuring/PopRoutine.lean
@@ -9,7 +9,6 @@ module
 public import Cslib.Computability.Machines.MultiTapeTuring.Basic
 public import Cslib.Computability.Machines.MultiTapeTuring.ListEncoding
 public import Cslib.Computability.Machines.MultiTapeTuring.WithTapes
-public import Cslib.Computability.Machines.MultiTapeTuring.TMWithAuxTapes
 
 namespace Turing
 
@@ -27,12 +26,12 @@ public lemma pop₁_eval_list {tapes : Fin 1 → List (List α)} :
   pop₁.eval_list tapes = .some (Function.update tapes 0 (tapes 0).tail) := by
   sorry
 
-public def pop {k : ℕ} (i : Fin k.succ) : MultiTapeTM k.succ (WithSep α) :=
+public def pop {k : ℕ} (i : Fin k) : MultiTapeTM k (WithSep α) :=
   pop₁.with_tapes [i].get (by intro x y; grind)
 
 @[simp, grind =]
-public theorem pop_eval_list {k : ℕ} {i : Fin k.succ}
-  {tapes : Fin k.succ → List (List α)} :
+public theorem pop_eval_list {k : ℕ} {i : Fin k}
+  {tapes : Fin k → List (List α)} :
   (pop i).eval_list tapes = .some (Function.update tapes i (tapes i).tail) := by
   have h_inj : [i].get.Injective := by intro x y; grind
   simp_all [pop]
